Tap

Isotope/Syntax/Intrinsic/Basic.lean
@@ -1,92 +1,132 @@
-import Mathlib.Init.Order.Defs
-import Mathlib.Data.Bool.Basic
-import Mathlib.Logic.Equiv.Defs
+import Isotope.Syntax.Intrinsic.LCtx
 
-inductive Ty (T: Type u)
-| base (X: T)
-| unit
-| bool
-| tensor (A B: Ty T)
+inductive GCtx (T: Type u) [HasLin T]: Type u
+  | df (Γ: Ctx T)
+  | cf (L: LCtx T)
 
-class HasLin (T: Type u) :=
-  aff: T → Bool
-  rel: T → Bool
+inductive Result (T: Type u) [HasLin T]: Type u
+  | term (x: Var T)
+  | label (L: LCtx T)
 
-instance Ty.instHasLin {T} [HasLin T]: HasLin (Ty T) where
-  aff := let rec aff
-    | base X => HasLin.aff X
-    | tensor A B => aff A && aff B
-    | _ => true
-    aff
-  rel := let rec rel
-    | base X => HasLin.rel X
-    | tensor A B => rel A && rel B
-    | _ => true
-    rel
+class InstructionSet (F: Type u) (T: Type v)
+  where
+  inst_ty: F -> Ty T -> Ty T -> Prop
+  inst_aff: F -> Ty T -> Ty T -> Prop
+  inst_rel: F -> Ty T -> Ty T -> Prop
+  inst_cen: F -> Ty T -> Ty T -> Prop
 
-structure Transparency where
-  aff: Bool
-  rel: Bool
 
-def HasLin.lin {T} [HasLin T] (t: T) (l: Transparency): Bool
-  := (l.aff → HasLin.aff t) ∧ (l.rel → HasLin.rel t)
+structure InstructionSet.inst {F: Type u} {T: Type v}
+  [HasLin T] [InstructionSet F T]
+  (f: F) (p: Bool) (q: Transparency) (A B: Ty T) where
+  well_typed: inst_ty f A B
+  inst_aff: (q.aff → inst_aff f A B)
+  insrt_rel: (q.rel → inst_rel f A B)
+  inst_cen: (p → inst_cen f A B)
 
-instance Transparency.instHasLin: HasLin Transparency where
-  aff := Transparency.aff
-  rel := Transparency.rel
+open InstructionSet
 
-instance Transparency.instPartialOrder: PartialOrder Transparency where
-  le l r := l.aff ≤ r.aff ∧ l.rel ≤ r.rel
-  le_refl := by simp
-  le_trans _ _ _ H H' := ⟨le_trans H.1 H'.1, le_trans H.2 H'.2⟩
-  le_antisymm _ _ H H'
-    := mk.injEq _ _ _ _ ▸ ⟨le_antisymm H.1 H'.1, le_antisymm H.2 H'.2⟩
+inductive Term {T: Type u} [HasLin T] (F: Type u) [InstructionSet F T]
+  : Ctx T -> Bool -> Ty T -> Transparency -> Type u
+  | var {Γ A q} (p) (v: Γ.var ⟨q, A⟩): Term F Γ p A q
+  | app {Γ} {f: F} {p A B} (Hf: inst f p q A B)
+    : Term F Γ p A q -> Term F Γ p B q
+  | pair {Γ Δ Ξ A B q}: Γ.ssplit Δ Ξ
+    -> Term F Δ true A q
+    -> Term F Ξ true B q
+    -> Term F Γ true (Ty.tensor A B) q
+  | unit (p) (v: Ctx.wk Γ []) (q): Term F Γ p Ty.unit q
+  | tt (p) (v: Ctx.wk Γ []) (q): Term F Γ p Ty.bool q
+  | ff (p) (v: Ctx.wk Γ []) (q): Term F Γ p Ty.bool q
+  | let1 {Γ Δ Ξ A B q} (p): Γ.ssplit Δ Ξ
+    -> Term F Ξ true A q
+    -> Term F (⟨⟨true, true⟩, A⟩::Δ) p B q
+    -> Term F Γ p B q
+  | let2 {Γ Δ Ξ A B C q} (p): Γ.ssplit Δ Ξ
+    -> Term F Ξ true (Ty.tensor A B) q
+    -> Term F (⟨⟨true, true⟩, A⟩::⟨⟨true, true⟩, B⟩::Δ) p C q
+    -> Term F Γ p C q
 
-theorem Transparency.le.aff {l r: Transparency}
-  : l ≤ r → l.aff → r.aff := And.left
+inductive NCfg {T: Type u} (F: Type u) [HasLin T] [InstructionSet F T]
+  : GCtx T -> LCtx T -> Type u
+  | br {Γ Δ Ξ A q L}:
+    Γ.ssplit Δ Ξ ->
+    Term F Ξ true A q ->
+    LCtx.join [⟨Δ, ⟨q, A⟩⟩] L ->
+    NCfg F (GCtx.df Γ) L
+  | ite {Γ Δ Ξ L}:
+    Γ.ssplit Δ Ξ ->
+    Term F Ξ true Ty.bool q ->
+    NCfg F (GCtx.df Δ) L ->
+    NCfg F (GCtx.df Δ) L ->
+    NCfg F (GCtx.df Γ) L
+  | let1 {Γ Δ Ξ p A q L}:
+    Γ.ssplit Δ Ξ ->
+    Term F Ξ p A q ->
+    NCfg F (GCtx.df (⟨⟨true, true⟩, A⟩::Δ)) L ->
+    NCfg F (GCtx.df Γ) L
+  | let2 {Γ Δ Ξ p A B q L}:
+    Γ.ssplit Δ Ξ ->
+    Term F Ξ p (Ty.tensor A B) q ->
+    NCfg F (GCtx.df (⟨⟨true, true⟩, A⟩::⟨⟨true, true⟩, B⟩::Δ)) L ->
+    NCfg F (GCtx.df Γ) L
+  | cfg {Γ L K}:
+    NCfg F (GCtx.df Γ) L ->
+    NCfg F (GCtx.cf L) K ->
+    NCfg F (GCtx.df Γ) K
+  | cfg_id (L):
+    NCfg F (GCtx.cf L) L
+  | cfg_def {Γ A q L K}:
+    NCfg F (GCtx.cf (⟨Γ, ⟨q, A⟩⟩::L)) K ->
+    NCfg F (GCtx.df Γ) K ->
+    NCfg F (GCtx.cf L) K
 
-theorem Transparency.le.rel {l r: Transparency}
-  : l ≤ r → l.rel → r.rel := And.right
+def Block {T: Type u} [HasLin T] (F: Type u) [InstructionSet F T]
+  (Γ: Ctx T) (L: LCtx T) := NCfg F (GCtx.df Γ) L
+def Cfg {T: Type u} [HasLin T] (F: Type u) [InstructionSet F T]
+  (L: LCtx T) (K: LCtx T) := NCfg F (GCtx.cf L) K
 
---TODO: add resource algebra to variables?
-structure Var (T: Type u) extends Transparency where
-  ty: Ty T
+inductive GBlock {T: Type u} (F: Type u) [HasLin T] [InstructionSet F T]
+  : Ctx T -> LCtx T -> Bool -> Type u
+  | br {Γ Δ Ξ A q L} (t):
+    Γ.ssplit Δ Ξ ->
+    Term F Ξ true A q ->
+    LCtx.join [⟨Δ, ⟨q, A⟩⟩] L ->
+    GBlock F Γ L t
+  | ite {Γ Δ Ξ L} (t):
+    Γ.ssplit Δ Ξ ->
+    Term F Ξ true Ty.bool q ->
+    GBlock F Δ L true ->
+    GBlock F Δ L true ->
+    GBlock F Γ L t
+  | let1 {Γ Δ Ξ p A q L t}:
+    Γ.ssplit Δ Ξ ->
+    Term F Ξ p A q ->
+    GBlock F (⟨⟨true, true⟩, A⟩::Δ) L t ->
+    GBlock F Γ L false
+  | let2 {Γ Δ Ξ p A B q L t}:
+    Γ.ssplit Δ Ξ ->
+    Term F Ξ p (Ty.tensor A B) q ->
+    GBlock F (⟨⟨true, true⟩, A⟩::⟨⟨true, true⟩, B⟩::Δ) L t ->
+    GBlock F Γ L false
 
-instance Var.instHasLin {T} [HasLin T]: HasLin (Var T) where
-  aff v := v.aff && HasLin.aff v.ty
-  rel v := v.rel && HasLin.rel v.ty
+def BBlock {T: Type u} (F: Type u) [HasLin T] [InstructionSet F T]
+  (Γ: Ctx T) (L: LCtx T) := GBlock F Γ L false
 
-instance Var.instPartialOrder {T}: PartialOrder (Var T) where
-  le l r := l.ty = r.ty ∧ l.toTransparency ≤ r.toTransparency
-  le_refl := by simp [le_refl]
-  le_trans _ _ _  | ⟨He, Ht⟩, ⟨He', Ht'⟩ => ⟨He.trans He', le_trans Ht Ht'⟩
-  le_antisymm x x' H H'
-    := mk.injEq _ _ _ _ ▸ ⟨le_antisymm H.2 H'.2, H.1⟩
+inductive SCfg {T: Type u} (F: Type u) [HasLin T] [InstructionSet F T]
+  : LCtx T -> LCtx T -> Type u
+  | cfg_id (L):
+    SCfg F L L
+  | cfg_def {Γ A q L K}:
+    SCfg F (⟨Γ, ⟨q, A⟩⟩::L) K ->
+    BBlock F Γ K ->
+    SCfg F L K
 
-theorem Var.le.aff {T} [HasLin T] {l r: Var T}
-  : l ≤ r → HasLin.aff l → HasLin.aff r
-  | ⟨He, Ht⟩ => by
-    simp only [HasLin.aff, He, Bool.and_eq_true, and_imp]
-    intro H H';
-    exact ⟨Ht.1 H, H'⟩
-
-theorem Var.le.rel {T} [HasLin T] {l r: Var T}
-  : l ≤ r → HasLin.rel l → HasLin.rel r
-  | ⟨He, Ht⟩ => by
-    simp only [HasLin.rel, He, Bool.and_eq_true, and_imp]
-    intro H H';
-    exact ⟨Ht.2 H, H'⟩
-
-structure Comp (T: Type u) extends Var T where
-  cen: Bool
-
-instance Comp.instHasLin {T} [HasLin T]: HasLin (Var T) where
-  aff v := v.aff && HasLin.aff v.ty
-  rel v := v.rel && HasLin.rel v.ty
-
-instance Comp.instPartialOrder {T}: PartialOrder (Comp T) where
-  le l r := l.toVar ≤ r.toVar ∧ l.cen ≤ r.cen
-  le_refl := by simp [le_refl]
-  le_trans _ _ _  | ⟨He, Ht⟩, ⟨He', Ht'⟩ => ⟨le_trans He He', le_trans Ht Ht'⟩
-  le_antisymm x x' H H'
-    := mk.injEq _ _ _ _ ▸ ⟨le_antisymm H.1 H'.1, le_antisymm H.2 H'.2⟩
+-- inductive Term.subst {T} [HasLin T]: Ctx T -> Ctx T -> Type
+--   | nil {Γ} (H: Ctx.wk Γ []): subst Γ []
+--   | cons {Θ ΘΓ Γ Θx x}
+--     (s: Ctx.ssplit Θ ΘΓ Θx)
+--     (HΘΓ: subst ΘΓ Γ)
+--     (HΘx: HasLin.lin Θx x.toTransparency)
+--     (t: Term Θx x)
+--     : subst Θ (x::Γ)
