Isotope/Syntax/Intrinsic/Ty.lean
@@ -1,0 +1,92 @@
+import Mathlib.Init.Order.Defs
+import Mathlib.Data.Bool.Basic
+import Mathlib.Logic.Equiv.Defs
+
+inductive Ty (T: Type u)
+| base (X: T)
+| unit
+| bool
+| tensor (A B: Ty T)
+
+class HasLin (T: Type u) :=
+  aff: T → Bool
+  rel: T → Bool
+
+instance Ty.instHasLin {T} [HasLin T]: HasLin (Ty T) where
+  aff := let rec aff
+    | base X => HasLin.aff X
+    | tensor A B => aff A && aff B
+    | _ => true
+    aff
+  rel := let rec rel
+    | base X => HasLin.rel X
+    | tensor A B => rel A && rel B
+    | _ => true
+    rel
+
+structure Transparency where
+  aff: Bool
+  rel: Bool
+
+def HasLin.lin {T} [HasLin T] (t: T) (l: Transparency): Bool
+  := (l.aff → HasLin.aff t) ∧ (l.rel → HasLin.rel t)
+
+instance Transparency.instHasLin: HasLin Transparency where
+  aff := Transparency.aff
+  rel := Transparency.rel
+
+instance Transparency.instPartialOrder: PartialOrder Transparency where
+  le l r := l.aff ≤ r.aff ∧ l.rel ≤ r.rel
+  le_refl := by simp
+  le_trans _ _ _ H H' := ⟨le_trans H.1 H'.1, le_trans H.2 H'.2⟩
+  le_antisymm _ _ H H'
+    := mk.injEq _ _ _ _ ▸ ⟨le_antisymm H.1 H'.1, le_antisymm H.2 H'.2⟩
+
+theorem Transparency.le.aff {l r: Transparency}
+  : l ≤ r → l.aff → r.aff := And.left
+
+theorem Transparency.le.rel {l r: Transparency}
+  : l ≤ r → l.rel → r.rel := And.right
+
+--TODO: add resource algebra to variables?
+structure Var (T: Type u) extends Transparency where
+  ty: Ty T
+
+instance Var.instHasLin {T} [HasLin T]: HasLin (Var T) where
+  aff v := v.aff && HasLin.aff v.ty
+  rel v := v.rel && HasLin.rel v.ty
+
+instance Var.instPartialOrder {T}: PartialOrder (Var T) where
+  le l r := l.ty = r.ty ∧ l.toTransparency ≤ r.toTransparency
+  le_refl := by simp [le_refl]
+  le_trans _ _ _  | ⟨He, Ht⟩, ⟨He', Ht'⟩ => ⟨He.trans He', le_trans Ht Ht'⟩
+  le_antisymm x x' H H'
+    := mk.injEq _ _ _ _ ▸ ⟨le_antisymm H.2 H'.2, H.1⟩
+
+theorem Var.le.aff {T} [HasLin T] {l r: Var T}
+  : l ≤ r → HasLin.aff l → HasLin.aff r
+  | ⟨He, Ht⟩ => by
+    simp only [HasLin.aff, He, Bool.and_eq_true, and_imp]
+    intro H H';
+    exact ⟨Ht.1 H, H'⟩
+
+theorem Var.le.rel {T} [HasLin T] {l r: Var T}
+  : l ≤ r → HasLin.rel l → HasLin.rel r
+  | ⟨He, Ht⟩ => by
+    simp only [HasLin.rel, He, Bool.and_eq_true, and_imp]
+    intro H H';
+    exact ⟨Ht.2 H, H'⟩
+
+structure Comp (T: Type u) extends Var T where
+  cen: Bool
+
+instance Comp.instHasLin {T} [HasLin T]: HasLin (Var T) where
+  aff v := v.aff && HasLin.aff v.ty
+  rel v := v.rel && HasLin.rel v.ty
+
+instance Comp.instPartialOrder {T}: PartialOrder (Comp T) where
+  le l r := l.toVar ≤ r.toVar ∧ l.cen ≤ r.cen
+  le_refl := by simp [le_refl]
+  le_trans _ _ _  | ⟨He, Ht⟩, ⟨He', Ht'⟩ => ⟨le_trans He He', le_trans Ht Ht'⟩
+  le_antisymm x x' H H'
+    := mk.injEq _ _ _ _ ▸ ⟨le_antisymm H.1 H'.1, le_antisymm H.2 H'.2⟩
